src/impl/TLS13.Connection.Core.fsti
@@ -80,9 +80,11 @@ type request_kind =
 let request_record_sequence_fits
   (kind:request_kind)
   (view:CL.connection_view)
+  (app_in:B.bytes)
   : prop =
   match kind with
-  | KSendApplicationData
+  | KSendApplicationData ->
+    U64.fits (view.CL.state.S.write_state.R.seq + S.application_data_record_count app_in)
   | KClose ->
     U64.fits (view.CL.state.S.write_state.R.seq + 1)
   | KReadApplicationData ->
@@ -158,7 +160,7 @@ requires
     B.length 'network_out0 == SZ.v network_out_cap /\
     B.length 'app_out0 == SZ.v app_out_cap /\
     view0.CL.state.S.phase == S.ApplicationData /\
-    request_record_sequence_fits kind view0 /\
+    request_record_sequence_fits kind view0 (Ghost.reveal 'app_in_bytes) /\
     request_buffers_match
       kind
       (Ghost.reveal 'network_in_bytes)
